

CSCE 222

## Homework 2

Jonathan Kalsky

Feb. 13 2026

### Contents

<b>1</b>	<b>Section 1.6</b>	<b>1</b>
<b>2</b>	<b>Section 1.7</b>	<b>3</b>
<b>3</b>	<b>Section 2.1</b>	<b>5</b>
<b>4</b>	<b>Section 2.2</b>	<b>6</b>

### 1 Section 1.6

#### Question 14

a)

p = "In the class"

q = "Owns a red convertible"

r = "Got a speeding ticket"

$\forall x(q(x) \rightarrow r(x))$  premise

$p(x) \wedge q(x)$  Premise

$q(x)$  Simplification

$r(x)$  Modus ponens

Due to linda, there is at least one person who has gotten a speeding ticket in this class

**b)**

$p$  = "Taken a course in discrete mathematics"

$q$  = "Can take a course in algorithms"

$\forall x(p(x) \rightarrow q(x))$

$p(M) \wedge p(A) \wedge p(R) \wedge p(V) \wedge p(K)$  Premise

$q(M) \wedge q(A) \wedge q(R) \wedge q(V) \wedge q(K)$  Modus Ponens

Because all 5 took discrete math, this implies all 5 are eligible for algorithms

**c)**

$p$  = "produced by John Sayles"

$q$  = "Is wonderful"

$\forall x(p(x) \rightarrow q(x))$

$p(Coal)$  Premise

$q(Coal)$  Modus Ponens

Because the movie about coal miners is produced by John Sayles, the movie is wonderful; thus, there is a wonderful movie about coal miners.

**d)**

$p$  = "Been to France"

$q$  = "Visited the Lovre"

$\forall x(p(x) \rightarrow q(x))$

$p(x)$  Premise

$q(x)$  Modus Ponens

## Question 24

The error is on step 3, because you cannot simplify  $P(c) \vee Q(c)$  to  $P(c)$

## FRQ

p = "There is an undeclared variable"

q = "There is a syntax error in the first five lines"

r = "There is a missing semicolon"

s = "Variable name is misspelled"

$q \rightarrow (r \vee s)$

$p \vee q$

$\neg r$  Premise

$\neg s$  Premise

$\neg(r \vee s) \rightarrow \neg q = (\neg r \wedge \neg s) \rightarrow \neg q$  Modus Tollens

$\neg q$

Given there is no missing semicolon or misspelled variable name, there is not a syntax error in the first 5 lines.

## 2 Section 1.7

## Question 18

$\forall m, n, k \in \mathbb{Z}, mn = 2k \iff mn$  is even. By definition.

$(m = 2k \wedge n = 2k+1) \vee (m = 2k+1 \wedge n = 2k) \rightarrow mn = (2(k(2k+1))) \vee (2(k(2k)))$

Through association,  $mn$  is even by definition.

$mn \in \mathbb{Z}$  under multiplication since  $k \in \mathbb{Z}$ .

Therefore, if  $m$  or  $n$  are even integers,  $mn$  is even.

## Question 20

$p = \text{"n is an integer"} \quad q = \text{"is even"}$

### a) By contraposition

$p(n) \wedge q(3n + 2) \rightarrow q(n)$  Premise

$\neg q(n) \rightarrow \neg p(n) \vee \neg q(3n + 2)$  Contraposition

$(3n + 2) = (3n + 2(1))$  Identity

$2(1)$  is even by definition. Even + Even = Even, Odd + Even = Odd

Since:  $2k + 2k = 2(2k)$  and  $(2k + 1) + (2k) = 2(2k) + 1$

By the same reduction,  $3n + 2 = 2(n+1) + n = n$

$\neg q(n) \equiv \neg q(3n + 2)$  By definition of even

This makes the condition true, and since the contrapositive is true, the original is true.

### b) By contradiction

$p(n) \wedge q(3n + 2) \rightarrow q(n)$  Premise

Assume  $\neg q(n)$  By Contradiction

$3n+2 = 3(2k+1) + 2 = 6k + 5 = 2(3k + 2) + 1$

This implies  $\neg q(3n + 2)$  which contradicts the premise

## Question 34

if rational  $x$  was equivalent to rational  $x/2$ , it could be written as  $x = \frac{p}{q}$  and  $x/2 = \frac{p}{q/2}$ , where  $q$  is just another integer.

Then,  $3x-1$  can also be written as  $\frac{3p}{q} - 1 = \frac{3p-q}{q}$

$x$  can take on any real number, so with different combinations of  $p$  and  $q$ ,

$x$  is rational  $\equiv x/2$  is rational  $\equiv 3x-1$  is rational

## FRQ

Prove:  $x \in \mathbb{Z}^+ \rightarrow (x = 2k \iff 7x + 4 = 2k | k \in \mathbb{Z}^+)$

$$7x+4 = 2(3x+2) + x$$

This implies  $7x+4$  is only a multiple of 2 if  $x$  is also a multiple of 2, where  $x$  is a positive integer.

## FRQ

$R =$  "The square root of any irrational number is irrational."

a)

$\neg R =$  "The square root of any irrational number is rational."

b)

prove:  $\sqrt{\text{irrational}} = \text{irrational}$

Assume opposite:  $\sqrt{\text{irrational}} = \text{rational}$

$\sqrt{\text{irrational}} = \frac{p}{q}$  Definition of a rational number

$$\text{irrational} = \left(\frac{p}{q}\right)^2$$

$p, q \in \mathbb{Z}$ , so  $\left(\frac{p}{q}\right)^2$  is likely to be rational, which is a contradiction.

By contradiction  $R$  is true, "The square root of any irrational number is irrational."

## 3 Section 2.1

### Question 46

Use proofs?

Multiplication of sets is not commutative: If  $A = (a_1, a_2)$  and  $B = (b_1, b_2)$

$A \times B$  is a set of  $a_1$  and  $a_2$  with all combinations of  $B$ , in that order. Therefore the order of multiplication matters, and the resulting set is not necessarily equivalent if switched.  $(A \times B) \times (C \times D)$  and  $A \times (B \times C) \times D$  are not the same.

## Question 48

Prove  $A \times B = A \times C \rightarrow B = C$

$A$ ,  $B$ , and  $C$  are nonempty sets | Premise

$A \times B = \{(a, b) \mid a \in A \wedge b \in B\}$  | Cartesian Product

$A \times C = \{(a, c) \mid a \in A \wedge c \in C\}$  | Cartesian Product

$\forall a, b, c ((a, b) = (a, c) \rightarrow b = c) \rightarrow B = C$  | Definition of Set Equality

## 4 Section 2.2

## Question 20

a)

$p$  = "element in  $A$ "  $q$  = "element in  $B$ "  $r$  = "element in  $C$ "

$(A \cup B \cup C) = (A \cup B) \cup C$  | Association Law

$(p \vee q) \vee r$  | Written as propositions

$(p \vee q) \rightarrow (p \vee q) \vee r$  | Tautological

Therefore  $(A \cup B) \equiv (A \cup B \cup C)$

b)

$A \cap B \cap C \equiv (A \cap B) \cap C$  | Association Law

$x \in (A \cap B \cap C) \iff x \in A \wedge x \in B \wedge x \in C$  | Meaning of Intersection

$x \in A \wedge x \in B \wedge x \in C \rightarrow x \in A \wedge x \in B$  | Simplification

$\therefore A \cap B \cap C \subseteq A \cap B$

**c)**

$$(A - B) - C \equiv (A - C) - B \mid \text{Commutative Law}$$

$$(A - C) - B \equiv \{\forall x(x \in (A - C) \wedge (A - C) - B)\} \mid \text{Equivalence of a set intersection}$$

$$\forall x(x \in (A - C) \wedge (A - C) - B \rightarrow \forall x(x \in (A - C)))$$

All elements of this set have to be in A-C, thus it is a subset of A-C, therefore

$$(A - B) - C \subseteq A - C$$

**d)**

$$\forall x(x \in (A - C) \rightarrow x \notin C) \mid \text{Definition of set subtraction}$$

$$\forall x(x \in (C - B) \rightarrow x \in C) \mid \text{Definition of set subtraction}$$

$\forall x \neg((x \in (A - C)) \wedge (x \in (C - B))) \rightarrow (A - C) \cap (C - B) = \emptyset$  | Since by definition of intersection, for all elements there are no elements existing in both sets, the resulting set is empty by definition of an empty set.

**e)**

$$(B - A) \cup (C - A) \equiv \{x \in B \mid x \notin A\} \cup \{x \in C \mid x \notin A\} \mid \text{Definition of Set Difference}$$

$$\equiv \{x \in B \cup C \mid x \notin A\} \mid \text{Definition of Set Union}$$

$$\equiv (B \cup C) \cap A^c \mid \text{Definition of a Complement}$$

$$\equiv (B \cup C) - A \mid \text{Definition of Set Difference}$$

$$\therefore (B - A) \cup (C - A) \equiv (B \cup C) - A$$